qa/lean/Ragu/Circuits/Element/AllocSquare.lean
@@ -9,48 +9,44 @@ structure Square (F : Type) where
   a_sq : F
 deriving ProvableStruct
 
-def main (hintReader : ProverHint (F p) → F p) (_input : Unit) :
+def main (hint : ProverEnvironment (F p) → F p) :
     Circuit (F p) (Var Square (F p)) := do
   let ⟨x, y, z⟩ ← Core.AllocMul.circuit
-    (fun hint =>
-      let a := hintReader hint
-      ⟨a, a, a * a⟩) ()
+    (fun env =>
+      let a := hint env
+      ⟨a, a, a * a⟩)
   assertZero (x - y)
   return ⟨x, z⟩
 
 def Assumptions (_input : Unit) (_data : ProverData (F p)) := True
 
-def ProverAssumptions (_input : Unit) (_data : ProverData (F p)) (_hint : ProverHint (F p)) := True
+def ProverAssumptions (_input : F p) (_data : ProverData (F p)) (_hint : ProverHint (F p)) := True
 
 def Spec (_input : Unit) (out : Square (F p)) (_data : ProverData (F p)) :=
   out.a_sq = out.a^2
 
-def ProverSpec (hintReader : ProverHint (F p) → F p)
-    (_input : Unit) (out : Square (F p)) (hint : ProverHint (F p)) :=
-  let a := hintReader hint
-  out.a = a ∧ out.a_sq = a^2
+def ProverSpec (input : F p) (out : Square (F p)) (_hint : ProverHint (F p)) :=
+  out.a = input ∧ out.a_sq = input^2
 
-instance elaborated (hintReader : ProverHint (F p) → F p) :
-    ElaboratedCircuit (F p) unit Square where
-  main := main hintReader
+instance elaborated :
+    ElaboratedCircuit (F p) (Unconstrained (F p)) Square where
+  main
   localLength _ := 3
 
-theorem soundness (hintReader : ProverHint (F p) → F p) :
-    GeneralFormalCircuit.Soundness (F p) (elaborated hintReader) Assumptions Spec := by
+theorem soundness :
+    GeneralFormalCircuit.WithHint.Soundness (F p) elaborated Assumptions Spec := by
   circuit_proof_start [Core.AllocMul.circuit, Core.AllocMul.Spec]
   obtain ⟨h_mul, h_eq⟩ := h_holds
-  have h_mul := h_mul trivial
   -- h_mul : x * y = z, h_eq : x - y = 0
   rw [add_neg_eq_zero] at h_eq
   -- Goal: z = x^2
   rw [← h_mul, h_eq]; ring
 
-theorem completeness (hintReader : ProverHint (F p) → F p) :
-    GeneralFormalCircuit.Completeness (F p) (elaborated hintReader)
-      ProverAssumptions (ProverSpec hintReader) := by
+theorem completeness :
+    GeneralFormalCircuit.WithHint.Completeness (F p) elaborated
+      ProverAssumptions ProverSpec := by
   circuit_proof_start [
-    Core.AllocMul.circuit, Core.AllocMul.Assumptions,
-    Core.AllocMul.ProverAssumptions, Core.AllocMul.ProverSpec
+    Core.AllocMul.circuit, Core.AllocMul.ProverSpec
   ]
   obtain ⟨_, hx, hy, hz⟩ := h_env
   constructor
@@ -60,14 +56,13 @@ theorem completeness (hintReader : ProverHint (F p) → F p) :
     refine ⟨hx, ?_⟩
     rw [hz]; ring
 
-def circuit (hintReader : ProverHint (F p) → F p) :
-    GeneralFormalCircuit (F p) unit Square :=
-  { elaborated hintReader with
+def circuit : GeneralFormalCircuit.WithHint (F p) (Unconstrained (F p)) Square :=
+  { elaborated with
     Assumptions := Assumptions,
     Spec,
     ProverAssumptions := ProverAssumptions,
-    ProverSpec := ProverSpec hintReader,
-    soundness := soundness hintReader,
-    completeness := completeness hintReader }
+    ProverSpec := ProverSpec,
+    soundness := soundness,
+    completeness := completeness }
 
 end Ragu.Circuits.Element.AllocSquare
